add skeletons for iterators in MutBucket

Impl/MutableBucket.i.dfy
@@ -2,6 +2,8 @@ include "../lib/DataStructures/tttree.i.dfy"
 include "KVList.i.dfy"
 include "KVListPartialFlush.i.dfy"
 include "../PivotBetree/Bounds.i.dfy"
+include "../PivotBetree/BucketIterator.i.dfy"
+
 //
 // Collects singleton message insertions efficiently, avoiding repeated
 // replacement of the immutable root Node. Once this bucket is full,
@@ -22,6 +24,7 @@ module MutableBucket {
   import opened Bounds
   import opened BucketWeights
   import opened NativeTypes
+  import BucketIterator
   import Pivots = PivotsLib
 
   type Key = Element
@@ -81,6 +84,9 @@ module MutableBucket {
     }
     tree := TTT.NonEmptyTree(ar[0 as uint64].1);
   }
+
+  type Iterator
+  function IIterator(it: Iterator) : BucketIterator.Iterator
 
   class MutBucket {
     var is_tree: bool;
@@ -173,10 +179,10 @@ module MutableBucket {
       forall i | 0 <= i < |s| :: s[i].Inv()
     }
 
-    static function I(s: MutBucket) : Bucket
-    reads s
+    function I() : Bucket
+    reads this
     {
-      s.Bucket
+      this.Bucket
     }
 
     static protected function ISeq(s: seq<MutBucket>) : (bs : seq<Bucket>)
@@ -187,12 +193,12 @@ module MutableBucket {
     decreases |s|
     {
       reveal_ReprSeq();
-      if |s| == 0 then [] else ISeq(DropLast(s)) + [I(Last(s))]
+      if |s| == 0 then [] else ISeq(DropLast(s)) + [Last(s).I()]
     }
 
     static lemma ISeqInduction(s: seq<MutBucket>)
     requires |s| > 0
-    ensures ISeq(s) == ISeq(DropLast(s)) + [I(Last(s))]
+    ensures ISeq(s) == ISeq(DropLast(s)) + [Last(s).I()]
 
     static predicate {:opaque} ReprSeqDisjoint(buckets: seq<MutBucket>)
     reads set i | 0 <= i < |buckets| :: buckets[i]
@@ -269,7 +275,7 @@ module MutableBucket {
     requires parent.Inv()
     requires InvSeq(children)
     requires WFBucketList(ISeq(children), pivots)
-    requires WeightBucket(I(parent)) <= MaxTotalBucketWeight() as int
+    requires WeightBucket(parent.I()) <= MaxTotalBucketWeight() as int
     requires WeightBucketList(ISeq(children)) <= MaxTotalBucketWeight() as int
     ensures newParent.Inv()
     ensures InvSeq(newChildren)
@@ -424,7 +430,7 @@ module MutableBucket {
       invariant w as int == WeightBucketList(bs[0..j]);
       {
         assert DropLast(bs[0..j+1]) == bs[0..j];
-        assert Last(bs[0..j+1]) == I(buckets[j]);
+        assert Last(bs[0..j+1]) == buckets[j].I();
         WeightBucketListSlice(bs, 0, j as int + 1);
 
         w := w + buckets[j].Weight;
@@ -492,5 +498,32 @@ module MutableBucket {
       }
       buckets' := ar[..];
     }
+
+    predicate WFIter(it: Iterator)
+    reads this, this.Repr
+    ensures this.WFIter(it) ==> this.Inv()
+    ensures this.WFIter(it) ==> BucketIterator.WFIter(I(), IIterator(it))
+
+    method IterStart() returns (it': Iterator)
+    requires Inv()
+    ensures this.WFIter(it')
+    ensures IIterator(it') == BucketIterator.IterStart(I())
+
+    method IterFindFirstGte(key: Key) returns (it': Iterator)
+    requires Inv()
+    ensures this.WFIter(it')
+    ensures IIterator(it') == BucketIterator.IterFindFirstGte(I(), key)
+
+    method IterFindFirstGt(key: Key) returns (it': Iterator)
+    requires Inv()
+    ensures this.WFIter(it')
+    ensures IIterator(it') == BucketIterator.IterFindFirstGt(I(), key)
+
+    method IterInc(it: Iterator) returns (it': Iterator)
+    requires Inv()
+    requires IIterator(it).next.Next?
+    requires this.WFIter(it)
+    ensures this.WFIter(it')
+    ensures IIterator(it') == BucketIterator.IterInc(I(), IIterator(it))
   }
 }
